src/QUIC.Impl.Lemmas.fst
@@ -1,86 +1,47 @@
 module QUIC.Impl.Lemmas
 include QUIC.Spec.Lemmas
 
-module G = FStar.Ghost
-module S = QUIC.Secret.Seq
-
-module U64 = FStar.UInt64
-module U32 = FStar.UInt32
-module U8 = FStar.UInt8
-
-module QS = QUIC.Spec
-module QSL = QUIC.Spec.Lemmas
-
-module Secret = QUIC.Secret.Int
-
 #set-options "--max_fuel 0 --max_ifuel 0"
 
 /// The usual sequence lemmas
 /// -------------------------
 
-let lemma_five_cuts (s: S.seq U8.t) (i1 i2 i3 i4 i5: nat) (s0 s1 s2 s3 s4 s5: S.seq U8.t): Lemma
-  (requires (
-    i1 <= S.length s /\
-    i2 <= S.length s /\
-    i3 <= S.length s /\
-    i4 <= S.length s /\
-    i5 <= S.length s /\
-    i1 <= i2 /\
-    i2 <= i3 /\
-    i3 <= i4 /\
-    i4 <= i5 /\
-    s0 `Seq.equal` S.slice s 0 i1 /\
-    s1 `Seq.equal` S.slice s i1 i2 /\
-    s2 `Seq.equal` S.slice s i2 i3 /\
-    s3 `Seq.equal` S.slice s i3 i4 /\
-    s4 `Seq.equal` S.slice s i4 i5 /\
-    s5 `Seq.equal` S.slice s i5 (S.length s)))
-  (ensures (
-    let open S in
-    s `equal` (s0 @| s1 @| s2 @| s3 @| s4 @| s5)))
+let lemma_five_cuts
+  s i1 i2 i3 i4 i5 s0 s1 s2 s3 s4 s5
 =
   ()
 
-let hash_is_keysized_ (a: QS.ha): Lemma
-  (ensures (QS.keysized a (Spec.Hash.Definitions.hash_length a)))
+let hash_is_keysized_
+  a
 =
   assert_norm (512 < pow2 61);
   assert_norm (512 < pow2 125)
 
-
-let lemma_slice s (i: nat { i <= S.length s }): Lemma
-  (ensures (s `S.equal` S.append (S.slice s 0 i) (S.slice s i (S.length s))))
+let lemma_slice
+  #t s i
 =
   ()
 
-let lemma_slice3 #a (s: S.seq a) (i j: nat): Lemma
-  (requires (i <= j /\ j <= S.length s))
-  (ensures (s `S.equal`
-    (S.slice s 0 i `S.append` S.slice s i j `S.append` S.slice s j (S.length s))))
+let lemma_slice3
+  #a s i j
 =
   ()
 
-let lemma_slice0 #a (s: S.seq a): Lemma (S.slice s 0 (S.length s) `S.equal` s) = ()
+let lemma_slice0
+  #a s
+= ()
 
-let lemma_slice1 #a (s: S.seq a) (i j: nat): Lemma
-  (requires (i <= j /\ j <= S.length s))
-  (ensures (S.slice s 0 j `S.equal`
-    (S.slice s 0 i `S.append` S.slice s i j)))
+let lemma_slice1
+  #a s i j
 =
   ()
 
 
 open FStar.Mul
 
-/// Lemmas about pointwise_op
-/// -------------------------------------------
-
 #push-options "--max_fuel 1 --z3rlimit 100"
-let pointwise_upd (#a: Type) f b1 b2 i pos (x: a): Lemma
-  (requires (S.length b2 + pos <= S.length b1 /\ i < pos))
-  (ensures (S.upd (QSL.pointwise_op f b1 b2 pos) i x `S.equal`
-    QSL.pointwise_op f (S.upd b1 i x) b2 pos))
-  (decreases (S.length b2))
+let pointwise_upd
+  #a f b1 b2 i pos x
 =
   calc (S.equal) {
     QSL.pointwise_op f (S.upd b1 i x) b2 pos;
@@ -126,15 +87,8 @@ let pointwise_upd (#a: Type) f b1 b2 i pos (x: a): Lemma
     S.upd (QSL.pointwise_op f b1 b2 pos) i x;
   }
 
-let rec pointwise_seq_map2 (#a: Type) (f: a -> a -> a) (s1 s2: S.seq a) (i: nat): Lemma
-  (requires (
-    let l = S.length s1 in
-    S.length s2 = l - i /\ i <= S.length s1))
-  (ensures (
-    let l = S.length s1 in
-    Spec.Loops.seq_map2 f (S.slice s1 i l) s2 `S.equal`
-    S.slice (QSL.pointwise_op f s1 s2 i) i l))
-  (decreases (S.length s2))
+let rec pointwise_seq_map2
+  #a f s1 s2 i
 =
   if S.length s2 = 0 then
     ()
@@ -181,11 +135,8 @@ let rec pointwise_seq_map2 (#a: Type) (f: a -> a -> a) (s1 s2: S.seq a) (i: nat)
 #pop-options
 
 #push-options "--max_fuel 2 --initial_fuel 2 --max_ifuel 1 --initial_ifuel 1"
-let rec and_inplace_commutative (s1 s2: S.seq U8.t): Lemma
-  (requires S.length s1 = S.length s2)
-  (ensures Spec.Loops.seq_map2 U8.logand s1 s2 `S.equal`
-    Spec.Loops.seq_map2 U8.logand s2 s1)
-  (decreases (S.length s1))
+let rec and_inplace_commutative
+  s1 s2
 =
   if S.length s1 = 0 then
     ()
@@ -199,13 +150,8 @@ let rec and_inplace_commutative (s1 s2: S.seq U8.t): Lemma
 #pop-options
 
 #push-options "--max_fuel 1"
-let rec seq_map2_xor0 (s1 s2: S.seq Secret.uint8): Lemma
-  (requires
-    S.length s1 = S.length s2 /\
-    s1 `S.equal` S.create (S.length s2) (Secret.to_u8 0uy))
-  (ensures
-    Spec.Loops.seq_map2 EverCrypt.CTR.xor8 s1 s2 `S.equal` s2)
-  (decreases (S.length s1))
+let rec seq_map2_xor0
+  s1 s2
 =
   if S.length s1 = 0 then
     ()
@@ -219,10 +165,8 @@ let rec seq_map2_xor0 (s1 s2: S.seq Secret.uint8): Lemma
 #pop-options
 
 #push-options "--max_fuel 2 --initial_fuel 2 --max_ifuel 1 --initial_ifuel 1"
-let upd_op_inplace (#a:Type) op (s: S.seq a) (x: a): Lemma
-  (requires S.length s > 0)
-  (ensures (S.upd s 0 (S.index s 0 `op` x) `S.equal`
-    QSL.pointwise_op op s (S.create 1 x) 0))
+let upd_op_inplace
+  #a op s x
 =
   ()
 #pop-options
@@ -232,11 +176,8 @@ let upd_op_inplace (#a:Type) op (s: S.seq a) (x: a): Lemma
 
 #push-options "--z3rlimit 16"
 #restart-solver
-let rec be_to_n_slice (s: S.seq U8.t) (i: nat): Lemma
-  (requires i <= S.length s)
-  (ensures FStar.Endianness.be_to_n (S.slice s i (S.length s)) =
-    FStar.Endianness.be_to_n s % pow2 (8 `op_Multiply` (S.length s - i)))
-  (decreases (S.length s))
+let rec be_to_n_slice
+  s i
 =
   FStar.Endianness.reveal_be_to_n s;
   if S.length s = 0 then
@@ -301,19 +242,7 @@ let rec be_to_n_slice (s: S.seq U8.t) (i: nat): Lemma
 #pop-options
 
 let n_to_be_lower
-  (len: nat)
-  (len' : nat)
-  (n: nat)
-: Lemma
-  (requires (
-    len <= len' /\
-    n < pow2 (8 * len)
-  ))
-  (ensures (
-    let open FStar.Endianness in
-    n < pow2 (8 * len') /\
-    n_to_be len n `FStar.Seq.equal` FStar.Seq.slice (n_to_be len' n) (len' - len) len'
-  ))
+  len len' n
 = let open FStar.Math.Lemmas in
   let open FStar.Endianness in
   pow2_le_compat (8 * len') (8 * len);
@@ -327,3 +256,117 @@ let n_to_be_lower
     QSL.index_n_to_be len' n (i + len' - len)
   in
   Classical.forall_intro phi
+
+
+#push-options "--z3rlimit 200"
+inline_for_extraction noextract
+let op_inplace'
+  (#t: Type)
+  (dst: B.buffer t)
+  (dst_len: Ghost.erased U32.t)
+  (src: B.buffer t)
+  (src_len: U32.t)
+  (ofs: U32.t)
+  (op: t -> t -> t)
+:
+  HST.Stack unit
+    (requires fun h0 ->
+      B.(all_live h0 [ buf dst; buf src ]) /\
+      B.disjoint dst src /\
+      B.length src == U32.v src_len /\
+      B.length dst == U32.v dst_len /\
+      B.length dst >= U32.v ofs + B.length src)
+    (ensures fun h0 _ h1 ->
+      B.(modifies (loc_buffer dst) h0 h1) /\
+      B.as_seq h1 dst `Seq.equal`
+        pointwise_op op (B.as_seq h0 dst) (B.as_seq h0 src) (U32.v ofs) /\
+      Seq.slice (B.as_seq h0 dst) 0 (U32.v ofs) `Seq.equal`
+        Seq.slice (B.as_seq h1 dst) 0 (U32.v ofs) /\
+      Seq.slice (B.as_seq h0 dst) (U32.v (ofs `U32.add` src_len)) (U32.v dst_len) `Seq.equal`
+      Seq.slice (B.as_seq h1 dst) (U32.v (ofs `U32.add` src_len)) (U32.v dst_len))
+=
+  let h0 = HST.get () in
+  let dst0 = B.sub dst 0ul ofs in
+  let dst1 = B.sub dst ofs src_len in
+  let dst2 = Ghost.hide (B.gsub dst (ofs `U32.add` src_len) (dst_len `U32.sub` (ofs `U32.add` src_len))) in
+  C.Loops.in_place_map2 dst1 src src_len op;
+  let h1 = HST.get () in
+  calc (Seq.equal) {
+    B.as_seq h1 dst;
+  (Seq.equal) { lemma_slice3 (B.as_seq h1 dst) (U32.v ofs) (U32.v (ofs `U32.add` src_len)) }
+    Seq.slice (B.as_seq h1 dst) 0 (U32.v ofs) `Seq.append`
+    (Seq.slice (B.as_seq h1 dst) (U32.v ofs) (U32.v (ofs `U32.add` src_len))) `Seq.append`
+    (Seq.slice (B.as_seq h1 dst) (U32.v (ofs `U32.add` src_len)) (B.length dst));
+  (Seq.equal) {}
+    Seq.slice (B.as_seq h0 dst) 0 (U32.v ofs) `Seq.append`
+    (Seq.slice (B.as_seq h1 dst) (U32.v ofs) (U32.v (ofs `U32.add` src_len))) `Seq.append`
+    (Seq.slice (B.as_seq h0 dst) (U32.v (ofs `U32.add` src_len)) (B.length dst));
+  (Seq.equal) { pointwise_seq_map2 op (B.as_seq h0 dst1) (B.as_seq h0 src) 0 }
+    Seq.slice (B.as_seq h0 dst) 0 (U32.v ofs) `Seq.append`
+    (pointwise_op op
+      (Seq.slice (B.as_seq h0 dst) (U32.v ofs) (U32.v (ofs `U32.add` src_len)))
+      (B.as_seq h0 src)
+      0) `Seq.append`
+    (Seq.slice (B.as_seq h0 dst) (U32.v (ofs `U32.add` src_len)) (B.length dst));
+  (Seq.equal) { pointwise_op_suff op (Seq.slice (B.as_seq h0 dst) 0 (U32.v ofs))
+    (Seq.slice (B.as_seq h0 dst) (U32.v ofs) (U32.v (ofs `U32.add` src_len)))
+    (B.as_seq h0 src)
+    (U32.v ofs) }
+    pointwise_op op
+      (Seq.append (Seq.slice (B.as_seq h0 dst) 0 (U32.v ofs))
+        (Seq.slice (B.as_seq h0 dst) (U32.v ofs) (U32.v (ofs `U32.add` src_len))))
+      (B.as_seq h0 src)
+      (U32.v ofs) `Seq.append`
+    (Seq.slice (B.as_seq h0 dst) (U32.v (ofs `U32.add` src_len)) (B.length dst));
+  (Seq.equal) { lemma_slice1 (B.as_seq h0 dst) (U32.v ofs) (U32.v (ofs `U32.add` src_len)) }
+    pointwise_op op
+      (Seq.slice (B.as_seq h0 dst) 0 (U32.v (ofs `U32.add` src_len)))
+      (B.as_seq h0 src)
+      (U32.v ofs) `Seq.append`
+    (Seq.slice (B.as_seq h0 dst) (U32.v (ofs `U32.add` src_len)) (B.length dst));
+  (Seq.equal) { pointwise_op_pref op
+    (Seq.slice (B.as_seq h0 dst) 0 (U32.v (ofs `U32.add` src_len)))
+    (Seq.slice (B.as_seq h0 dst) (U32.v (ofs `U32.add` src_len)) (B.length dst))
+    (B.as_seq h0 src)
+    (U32.v ofs)
+  }
+    pointwise_op op
+      (Seq.slice (B.as_seq h0 dst) 0 (U32.v (ofs `U32.add` src_len)) `Seq.append`
+      (Seq.slice (B.as_seq h0 dst) (U32.v (ofs `U32.add` src_len)) (B.length dst)))
+      (B.as_seq h0 src)
+      (U32.v ofs);
+  (Seq.equal) { lemma_slice (B.as_seq h0 dst) (U32.v (ofs `U32.add` src_len)) }
+    pointwise_op op
+      (B.as_seq h0 dst)
+      (B.as_seq h0 src)
+      (U32.v ofs);
+  }
+#pop-options
+
+let op_inplace
+  #t dst src src_len ofs op
+= op_inplace' dst (B.len dst) src src_len ofs op
+
+let secret_and_inplace_eq
+  b1 b2 pos
+= let f
+    (i: nat {i < S.length b1})
+  : Lemma
+    (S.index (S.seq_reveal (secret_and_inplace b1 b2 pos)) i == S.index (and_inplace (S.seq_reveal b1) (S.seq_reveal b2) pos) i)
+  =
+    pointwise_index (Secret.logand #Secret.U8 #Secret.SEC) b1 b2 i pos;
+    pointwise_index U8.logand (S.seq_reveal b1) (S.seq_reveal b2) i pos
+  in
+  Classical.forall_intro f
+
+let secret_xor_inplace_eq
+  b1 b2 pos
+= let f
+    (i: nat {i < S.length b1})
+  : Lemma
+    (S.index (S.seq_reveal (secret_xor_inplace b1 b2 pos)) i == S.index (xor_inplace (S.seq_reveal b1) (S.seq_reveal b2) pos) i)
+  =
+    pointwise_index (Secret.logxor #Secret.U8 #Secret.SEC) b1 b2 i pos;
+    pointwise_index U8.logxor (S.seq_reveal b1) (S.seq_reveal b2) i pos
+  in
+  Classical.forall_intro f
